theories/ftlr/ftlr_base.v
@@ -21,15 +21,15 @@ Section fundamental.
   Definition ftlr_instr
     (lregs : leibnizO LReg) (p : Perm)
         (b e a : Addr) (v : Version) (lw : LWord) (i: instr) (P : D) :=
-      p = RX ∨ p = RWX
+    custom_enclave_contract_gen
+    -> p = RX ∨ p = RWX
     → (∀ x : RegName, is_Some (lregs !! x))
     → isCorrectLPC (LCap p b e a v)
     → (b <= a)%a ∧ (a < e)%a
     → decodeInstrWL lw = i
-    → (□ custom_enclave_contract_gen ∗ custom_enclave_inv)
+    -> custom_enclave_inv
     (* Loeb induction hypothesis, but only for those assumptions that change in the recursive step *)
     -∗ □ ▷ (∀ lregs' p' b' e' a' v',
-              £ 1 -∗
              full_map lregs'
           -∗ (∀ (r1 : RegName) (lv : LWord),
               ⌜r1 ≠ PC⌝ → ⌜lregs' !! r1 = Some lv⌝ → (fixpoint interp1) lv)
@@ -49,7 +49,6 @@ Section fundamental.
                else emp)
             ∗ (persistent_cond P) (* P v ⊢ P v ∗ P v *)
 
-    -∗ £ 1
     -∗ na_own logrel_nais ⊤ (* same as the Loeb induction cond: knowledge about the existence of nonatomic invariants *)
     -∗ (a,v) ↦ₐ lw (* points-to for the address of the PC cap *) (* as a consequence of (1) *)
     -∗ ▷ P lw (* as a consequence of (1) *)
